perf(VMProm): refactor the TLB
This is a quite big refactor, however more than half the diff in 
VMPromising.v is just moving the TState after the TLB.

The main gist is that now the TLB is part of the TState for performance,
although it can be recomputed from the register and memory state at any point.
The TLB also contains information about all timestamps instead of just
one.

The 3 BBM mode are gone, and the BBM checker is either on or off.
Entries that a not-present can't be in conflict. If that is important
for proofs, the proof should have a precondition that all page table are
present.

Extraction/archsem.ml
@@ -66,15 +66,13 @@ module Arm = struct
         UMPromising.coq_UMPromising_opmodel_pf isem (Z.of_int nth)
     end)
 
-  module BBM = VMPromising.BBM
-
   module VMProm = OpModel.Of_coq (struct
-      type config = BBM.param
+      type config = bool
 
-      let default_config = BBM.Off
+      let default_config = false
 
-      let opmodel bbm_param isem ~nth =
-        VMPromising.coq_VMPromising_opmodel_pf bbm_param isem (Z.of_int nth)
+      let opmodel bbm isem ~nth =
+        VMPromising.coq_VMPromising_opmodel_pf bbm isem (Z.of_int nth)
     end)
 end
 
